\documentclass{article}
\usepackage{mathtools}
\begin{document}
Compare F.2 with F.8
\[
\tag{F.2}
C_D S=C_{D,wing}S(1+K_{wing}C_L^2)+C{D,fuse}S_{fuse}\left(1+K_{fuse}\alpha_{deg}^2\right)
\]
...
\[
\tag{F.8}
\frac{1}{e}=(1+\delta)+\pi AR C_{D,wing}K_{wing}+\pi C_{D,fuse}K_{fuse}\frac{(AR+3)^2}{0.12 AR}\frac{S_{fuse}}{S}
\]
\[
\alpha_{deg} = C_L\frac{\mathrm{d}\alpha_{deg}}{\mathrm{d}C_L}
\]
Substitute into F.2
\[
C_D S=C_{D,wing}S(1+K_{wing}{C_L}^2)+C{D,fuse}S_{fuse}\left(1+K_{fuse}\left({C_L\frac{\mathrm{d}\alpha_{deg}}{\mathrm{d}C_L}}\right)^2\right)
\]
Solve F.1 for $C_L^2$ and substitute into formula
\[
\tag{F.1}
C_D S = \left(C_{D,0}+\frac{C_L^2}{\pi eAR}\right)S
\]
\[
\frac{C_D S}{S} = C_{D,0}+\frac{C_L^2}{\pi eAR}
\]
\[
\frac{C_D S}{S}-C_{D,0} = \frac{C_L^2}{\pi eAR}
\]
\[
\frac{C_L^2}{\pi eAR} = \frac{C_D S}{S}-C_{D,0}
\]
\[
C_L^2 = {\pi eAR}\left(\frac{C_D S}{S}-C_{D,0}\right)
\]
\end{document}
